src/crypto/poly1305/x64/X64.Poly1305.Spec_s.fst
@@ -13,7 +13,7 @@ let nat128_max = 0x100000000000000000000000000000000
 let _ = assert_norm (pow2 128 = nat128_max) 
 type nat128 = x:int{0 <= x && x < nat128_max}
 
-let modp(x:int):int =
+let modp'(x:int):int =
   x % (nat128_max * 4 - 5)
 
 let and128 (x:nat128) (y:nat128) :nat128 =
@@ -24,7 +24,7 @@ let rec poly1305_hash_blocks (h:int) (pad:int) (r:int) (inp:int->nat128) (i:int)
   else
     let kk = k - 16 in
     let hh = poly1305_hash_blocks h pad r inp i kk in
-    modp ((hh + pad + inp kk) * r)
+    modp' ((hh + pad + inp kk) * r)
 
 let poly1305_hash (key_r:nat128) (key_s:nat128) (inp:int->nat128) (start:int) (len:nat) :int =
   let r = logand #128 key_r 0x0ffffffc0ffffffc0ffffffc0fffffff in
@@ -37,5 +37,5 @@ let poly1305_hash (key_r:nat128) (key_s:nat128) (inp:int->nat128) (start:int) (l
   else
     let k = start + 16 * nBlocks in
     let padLast = pow2(nExtra * 8) in
-    let hLast = modp ((hBlocks + padLast + ((inp k) % padLast)) * r) in
+    let hLast = modp' ((hBlocks + padLast + ((inp k) % padLast)) * r) in
     (hLast + key_s) % nat128_max
